wip determined approx

Core/Metatheory/Determined.lean
@@ -37,32 +37,280 @@ theorem determined_progress :
   sorry
 
 -- Syntactic approximation of determined
+
+
 def ExistsUnique {α : Sort u} (p : α → Prop) := ∃ x, p x ∧ ∀ y, p y → y = x
 
-def Trace : Type := List String
+inductive GuardTraceElem where
+| bound : String -> Nat -> GuardTraceElem
+| applied : String -> String -> GuardTraceElem
 
-inductive InstTrace (G : List Global) : Term -> Trace -> Prop where
+@[simp]
+def GuardTraceElem.contains (i : Nat) : GuardTraceElem -> Bool
+| bound _ n => i = n
+| applied _ _ => false
+
+@[simp]
+def GuardTraceElem.rmap (_ : Endo Ren) (r : Ren) : GuardTraceElem -> GuardTraceElem
+| bound x n => bound x (r n)
+| applied x y => applied x y
+
+instance : RenMap GuardTraceElem where
+  rmap := GuardTraceElem.rmap
+
+@[simp]
+def GuardTraceElem.from_act (x : String) (n : Nat) (a : Subst.Action Term) : GuardTraceElem :=
+  match a with
+  | re k => bound x k
+  | su t =>
+    match t.spine with
+    | some (y, _) => applied x y
+    | none => bound x n
+
+@[simp]
+def GuardTraceElem.smap (_ : Endo (Subst Term)) (σ : Subst Term) : GuardTraceElem -> GuardTraceElem
+| bound x n => from_act x n (σ n)
+| applied x y => applied x y
+
+instance : SubstMap GuardTraceElem Term where
+  smap := GuardTraceElem.smap
+
+@[simp]
+theorem GuardTraceElem.subst_bound :
+  (GuardTraceElem.bound x n)[σ:Term] = from_act x n (σ n)
+:= by simp [Subst.apply, SubstMap.smap]
+
+@[simp]
+theorem GuardTraceElem.subst_applied :
+  (GuardTraceElem.applied x y)[σ:Term] = .applied x y
+:= by simp [Subst.apply, SubstMap.smap]
+
+abbrev GuardTrace := List GuardTraceElem
+
+-- def GuardTrace.empty : GuardTrace := λ _ => none
+
+-- def GuardTrace.update (i : Nat) (x : String) (g : GuardTrace) : GuardTrace
+-- | n => if n = i then x else g n
+
+-- def GuardTrace.cons (x : String) (g : GuardTrace) : GuardTrace
+-- | 0 => x
+-- | n + 1 => g n
+
+-- def GuardTrace.skip (g : GuardTrace) : GuardTrace
+-- | 0 => none
+-- | n + 1 => g n
+
+-- def Trace : Type := List String
+
+-- def get_guard_pattern (x : Nat) : Term -> Option String
+-- | λ[_] t => get_guard_pattern (x + 1) t
+-- | Λ[_] t => get_guard_pattern (x + 1) t
+-- | .guard p #y t => do
+--   let (hd, _) <- p.spine
+--   if x = y then hd else get_guard_pattern x t
+-- | .guard _ _ t => get_guard_pattern x t
+-- | _ => none
+
+-- def OpenValue (G : List Global) (t : Term) : Prop := sorry
+
+-- 1. Need a context of free vars that tracks requirements on the substitution
+-- 2. Need a context for outer guards that tracks what trace has been substituted for that guard
+-- 3. Seems like you need two separate traces: the open lambda traces and the guard traces
+--    as you substitute, the open lambda trace gets propagated into the guard trace
+
+inductive InstTrace (G : List Global) : List Kind -> List Ty -> Term -> GuardTrace -> Prop where
 | base :
   t.Determined ->
-  InstTrace G t []
+  InstTrace G Δ Γ t []
 | lam :
-  InstTrace G t tr ->
-  InstTrace G (λ[A] t) tr
+  InstTrace G Δ (A::Γ) t (tr.map (·[+1:Term])) ->
+  InstTrace G Δ Γ (λ[A] t) tr
 | tlam :
-  InstTrace G t tr ->
-  InstTrace G (Λ[K] t) tr
-| guard_inner :
-  p.spine = some (d, sp) ->
-  InstTrace G t tr ->
-  InstTrace G (.guard p #x t) (d::tr)
-| guard_outer :
-  p.spine = some (d, sp1) ->
-  s.spine = some (y, sp2) ->
-  InstTrace G t tr ->
-  InstTrace G (.guard p s t) tr
+  InstTrace G (K::Δ) Γ t tr ->
+  InstTrace G Δ Γ (Λ[K] t) tr
+| guard_bound {Γ : List Ty} :
+  Γ[x]? = some A ->
+  A.spine = some (Ax, spA) ->
+  is_opent G Ax ->
+  p.spine = some (px, sp) ->
+  InstTrace G Δ Γ t tr ->
+  (.bound px x)::tr = tru ->
+  InstTrace G Δ Γ (.guard p #x t) tru
+| guard_applied :
+  p.spine = some (px, sp1) ->
+  s.spine = some (sx, sp2) ->
+  InstTrace G Δ Γ t tr ->
+  (.applied px sx)::tr = tru ->
+  InstTrace G Δ Γ (.guard p s t) tru
+
+-- inductive InstGuardPreamble (G : List Global) : List Kind -> List Ty -> Trace -> Term -> GuardTrace -> Prop where
+-- | base :
+--   t.Determined ->
+--   InstGuardPreamble G Δ Γ [] t .empty
+-- | lam :
+--   InstGuardPreamble G Δ (A::Γ)  tr t gtr.skip ->
+--   InstGuardPreamble G Δ Γ tr (λ[A] t) gtr
+-- | tlam :
+--   InstGuardPreamble G (K::Δ) Γ tr t gtr ->
+--   InstGuardPreamble G Δ Γ tr (Λ[K] t) gtr
+-- | guard_bound {Γ : List Ty} :
+--   Γ[x]? = some A ->
+--   A.spine = some (z, spA) ->
+--   is_opent G z ->
+--   p.spine = some (y, sp) ->
+--   gtr.update x y = gtru ->
+--   InstGuardPreamble G Δ Γ tr t gtr ->
+--   InstGuardPreamble G Δ Γ tr (.guard p #x t) gtru
+-- | guard :
+--   s.spine = some (y, sp) ->
+--   InstGuardPreamble G Δ Γ tr t gtr ->
+--   y::tr = tru ->
+--   InstGuardPreamble G Δ Γ tru (.guard p s t) gtr
+
+theorem InstTrace.subst {σ : Subst Term} :
+  (∀ i k, σ i = re k -> Γ[i]? = Γ'[k]?) ->
+  (∀ i b, σ i = su b -> b.Determined) ->
+  (∀ i b, σ i = su b -> tr.any (GuardTraceElem.contains i) -> b.spine.isSome) ->
+  InstTrace G Δ Γ t tr ->
+  InstTrace G Δ Γ' t[σ] (tr.map (·[σ:Term]))
+:= by
+  intro h1 h2 h3 j
+  induction j generalizing Γ' σ <;> simp
+  case base =>
+    sorry
+  case lam j ih =>
+    simp at ih
+    sorry
+  case tlam j ih =>
+    sorry
+  case guard_bound x A Ax spA px sp Δ t tr tru p Γ j1 j2 j3 j4 j5 j6 ih =>
+    subst j6; simp
+    have lem1 : p[σ].spine = some (px, sp.map (·[σ:Term])) := by sorry
+    replace ih := ih h1 h2 (by {
+      intro i b q1 q2
+      apply h3 i b q1
+      simp [*]
+    })
+    generalize zdef : σ x = z at *
+    cases z <;> simp
+    case re k =>
+      have lem2 : Γ'[k]? = some A := by sorry
+      apply guard_bound lem2 j2 j3 lem1 ih rfl
+    case su b =>
+      generalize wdef : b.spine = w at *
+      cases w
+      case some w =>
+        rcases w with ⟨y, ysp⟩; simp
+        apply guard_applied lem1 wdef ih rfl
+      case none =>
+        simp; exfalso
+        replace h3 := h3 _ _ zdef (by simp)
+        rw [wdef] at h3; simp at h3
+  case guard_applied px sp1 sx sp2 Δ Γ t tr tru p s j1 j2 j3 j4 ih =>
+    subst j4; simp
+    have lem1 : p[σ].spine = some (px, sp1.map (·[σ:Term])) := by sorry
+    have lem2 : s[σ].spine = some (sx, sp2.map (·[σ:Term])) := by sorry
+    replace ih := ih h1 h2 h3
+    apply guard_applied lem1 lem2 ih rfl
+
+-- theorem InstGuardPreamble.subst {σ : Subst Term} :
+--   List.Sublist tr tr' ->
+--   (∀ i k, σ i = re k -> gtr i = gtr' k ∧ Γ[i]? = Γ'[k]?) ->
+--   (∀ i t, σ i = su t -> gtr' i = none ∧ t.Determined) ->
+--   InstGuardPreamble G Δ Γ tr t gtr ->
+--   InstGuardPreamble G Δ' Γ' tr' t[σ] gtr'
+-- := by
+--   intro h1 h2 h3 j
+--   induction j generalizing σ Γ' Δ' <;> try simp
+--   case base =>
+--     have lem1 : gtr' = .empty := by sorry
+--     have lem2 : tr' = [] := by sorry
+--     subst lem1 lem2
+--     apply base
+--     sorry
+--   case lam j ih =>
+--     apply lam
+--     sorry
+--   case tlam j ih =>
+--     apply tlam
+--     sorry
+--   case guard_bound x A z spA y sp gtru Δ tr t gtr p Γ j1 j2 j3 j4 j5 j6 ih =>
+--     generalize zdef : σ x = z at *
+--     cases z <;> simp
+--     case re k =>
+--       obtain ⟨q1, q2⟩ := h2 x k zdef
+--       have lem1 : p[σ].spine = some (y, sp.map (·[σ:Term])) := by sorry
+--       apply guard_bound
+--       rw [<-q2]; exact j1
+--       apply j2; apply j3
+--       apply lem1
+--       repeat sorry
+--     case su w =>
+
+--       sorry
+--   case guard y sp Δ Γ tr t gtr tru p s j1 j2 j3 ih =>
+--     have lem1 : s[σ].spine = some (y, sp.map (·[σ:Term])) := by sorry
+--     apply guard lem1
+--     repeat sorry
+
+-- inductive InstTrace (G : List Global) : List Kind -> List Term -> Trace -> Term -> Trace -> Prop where
+-- | base :
+--   InstGuardPreamble G Δ Γ sptr t gtr
+
+-- inductive InstTrace (G : List Global) : List (Term -> Prop) -> Term -> Trace -> Prop where
+-- | base :
+--   InstGuardPreamble sptr t gtr ->
+--   InstTrace G [] t []
+-- | lam_closed :
+--   (A.spine = none ∨ (∃ x sp, A.spine = some (x, sp) ∧ ¬ is_opent G x)) ->
+--   InstTrace G (Term.Determined::ξ) t tr ->
+--   InstTrace G ξ (λ[A] t) tr
+-- | lam_open :
+--   A.spine = some (x, sp) ->
+--   is_opent G x ->
+--   get_guard_pattern 0 t = some d ->
+--   InstTrace G (OpenValue G::ξ) t tr ->
+--   InstTrace G ξ (λ[A] t) (d::tr)
+-- | tlam :
+--   InstTrace G ((λ _ => True)::ξ) t tr ->
+--   InstTrace G ξ (Λ[K] t) tr
+
+-- theorem InstTrace.subst (σ : Subst Term) :
+--   (∀ i, Term.Determined (σ i)) ->
+--   InstTrace G ξ t tr ->
+--   InstTrace G ξ t[σ] tr
+-- := by
+--   intro h j
+--   induction j generalizing σ
+--   case base => sorry
+--   case lam_closed => sorry
+--   case lam_open j1 j2 j3 j4 ih =>
+--     simp; apply lam_open j1 j2 sorry
+--     sorry -- by ih
+--   case tlam ih =>
+--     simp
+--     sorry
+--   case guard_inner j ih =>
+--     simp
+--     sorry
+--   case guard_outer => sorry
 
 
-
+-- inductive SpineTrace : Term -> List SpineElem -> Prop where
+-- | nil : t.Determined -> SpineTrace t []
+-- | type :
+--   SpineTrace b[su a::+0:Ty] tl ->
+--   SpineTrace (Λ[K] b) (.type a :: tl)
+-- | term :
+--   SpineTrace b[su a::+0] tl ->
+--   SpineTrace (λ[A] b) (.term a :: tl)
+-- | oterm :
+--   SpineTrace b[su a::+0] tl ->
+--   SpineTrace (λ[A] b) (.oterm a :: tl)
+-- | guard_matched :
+--   p.spine = some (x, sp1) ->
+--   s.spine = some (x, sp2) ->
+--   SpineTrace (.guard p s t) tl
 -- inductive InstTrace (G : List Global) : Term -> Trace -> Prop where
 -- | body : t.Determined -> InstTrace G t []
 -- | lam_open :
@@ -78,55 +326,55 @@ inductive InstTrace (G : List Global) : Term -> Trace -> Prop where
 --   InstTrace G c tr ->
 --   InstTrace G (.guard p s c) tr
 
-inductive SpineTrace : List SpineElem -> Trace -> Prop where
-| nil : SpineTrace [] []
-| type : SpineTrace tl tr -> SpineTrace (.type a :: tl) tr
-| term :
-  a.Determined ->
-  SpineTrace tl tr ->
-  SpineTrace (.term a :: tl) tr
-| oterm :
-  a.Determined ->
-  a.spine = some (x, sp) ->
-  SpineTrace tl tr ->
-  SpineTrace (.oterm a :: tl) (x::tr)
+-- inductive SpineTrace : List SpineElem -> Trace -> Prop where
+-- | nil : SpineTrace [] []
+-- | type : SpineTrace tl tr -> SpineTrace (.type a :: tl) tr
+-- | term :
+--   a.Determined ->
+--   SpineTrace tl tr ->
+--   SpineTrace (.term a :: tl) tr
+-- | oterm :
+--   a.Determined ->
+--   a.spine = some (x, sp) ->
+--   SpineTrace tl tr ->
+--   SpineTrace (.oterm a :: tl) (x::tr)
 
-def Saturated (G : List Global) : Prop :=
-  ∀ x insts,
-  instances x G = insts ->
-  sorry
+-- def Saturated (G : List Global) : Prop :=
+--   ∀ x insts,
+--   instances x G = insts ->
+--   sorry
 
-theorem inst_red_trace_agree :
-  InstTrace G t tr ->
-  SpineTrace sp tr ->
-  sp.length ≥ B.arity ->
-  G&[],[] ⊢ t : B ->
-  G&[],[] ⊢ t.apply sp : T ->
-  ∃ t', Star (Red G) (t.apply sp) t' ∧ t'.Determined
-:= by
-  intro j1 j2 h j3 j4
-  induction j2 generalizing t B T
-  case nil => sorry
-  case term => sorry
-  case oterm x sp tl tr a q1 q2 j ih =>
-    cases j1
-    case lam => sorry
-    case tlam => sorry -- impossible
-    case guard_inner => sorry -- impossible
-    case guard_outer d sp1 y sp2 t p s q3 q4 j1 =>
+-- theorem inst_red_trace_agree :
+--   InstTrace G t tr ->
+--   SpineTrace sp tr ->
+--   sp.length ≥ B.arity ->
+--   G&[],[] ⊢ t : B ->
+--   G&[],[] ⊢ t.apply sp : T ->
+--   ∃ t', Star (Red G) (t.apply sp) t' ∧ t'.Determined
+-- := by
+--   intro j1 j2 h j3 j4
+--   induction j2 generalizing t B T
+--   case nil => sorry
+--   case term => sorry
+--   case oterm x sp tl tr a q1 q2 j ih =>
+--     cases j1
+--     case lam => sorry
+--     case tlam => sorry -- impossible
+--     case guard_inner => sorry -- impossible
+--     case guard_outer d sp1 y sp2 t p s q3 q4 j1 =>
 
-      sorry
-  case type tl tr A j ih =>
-    cases j1
-    case base j1 => sorry -- already determined
-    case lam => sorry -- impossible
-    case tlam t K j1 =>
-      simp [Term.apply] at *
-      sorry
-    case guard_inner => sorry -- impossible
-    case guard_outer d sp1 y sp2 t p s q1 q2 j1 =>
+--       sorry
+--   case type tl tr A j ih =>
+--     cases j1
+--     case base j1 => sorry -- already determined
+--     case lam => sorry -- impossible
+--     case tlam t K j1 =>
+--       simp [Term.apply] at *
+--       sorry
+--     case guard_inner => sorry -- impossible
+--     case guard_outer d sp1 y sp2 t p s q1 q2 j1 =>
 
-      sorry
+--       sorry
 
 -- theorem inst_red_trace_disagree :
 --   InstTrace t tr1 ->
